Q2 implementation + refinement(mostly)

HeapInsert.dfy
@@ -1,11 +1,238 @@
-// include "CCPR191-HeapSort-complete-30Dec18.dfy"
+include "CCPR191-HeapSort-complete-30Dec18.dfy"
 
-// method HeapInsert(a: array<int>, heapsize: nat, x: int)
-// 	requires heapsize < a.Length
-// 	requires hp(a[..], heapsize)
-// 	ensures hp(a[..], heapsize+1)
-// 	ensures multiset(a[..heapsize+1]) == multiset(old(a[..heapsize])+[x])
-// 	modifies a
-// {
+predicate HeapExceptK(a : seq<int>, heapsize : nat, k : nat)
+    requires heapsize <= |a|
+{
+    ph(a, IndexSet(0, heapsize) - {k})
+}
 
-// }
+predicate Inv(a : seq<int>, heapsize : nat, i : nat, setToBe : multiset<int>)
+    //requires heapsize <= |a|
+{
+    heapsize <= |a| &&
+    HeapExceptK(a, heapsize, i) &&
+    0 <= i < heapsize <= |a| &&
+    multiset(a[..heapsize]) == setToBe &&
+    forall j :: 0 <= j < heapsize && AncestorIndex(i, j) ==> a[i] >= a[j]
+}
+
+method HeapInsert(a: array<int>, heapsize: nat, x: int)
+	requires heapsize < a.Length
+	requires hp(a[..], heapsize)
+	ensures hp(a[..], heapsize+1)
+	ensures multiset(a[..heapsize+1]) == multiset(old(a[..heapsize])+[x])
+	modifies a
+{
+    // assingment
+    AddXToLeaf(a, heapsize, x);
+    a[heapsize] := x;
+
+    // introduce logical constant
+    ghost var setToBe := multiset(old(a[..heapsize])+[x]);
+    
+    SiftLastItem(a, heapsize + 1, setToBe);
+}
+
+method SiftLastItem(a : array<int>, heapsize:nat,  ghost setToBe : multiset<int>)
+    requires 0 < heapsize <= a.Length
+	requires hp(a[..], heapsize - 1)
+    requires multiset(a[..heapsize]) == setToBe
+
+    ensures hp(a[..], heapsize)
+    ensures multiset(a[..heapsize]) == setToBe
+	modifies a
+    {
+        WeakenPrecondForIteration(a, heapsize, setToBe);
+        var i:= SiftLastItem_Iterate(a, heapsize, heapsize - 1, setToBe);
+        StrengthenPostFromIteration(a, heapsize, setToBe, i);
+    }
+
+lemma AddXToLeaf(a : array<int>, heapsize:nat, itemToAdd : int)
+    requires heapsize < a.Length
+	requires hp(a[..], heapsize)
+    ensures multiset(a[..heapsize+1][heapsize := itemToAdd][..heapsize + 1]) ==
+            multiset(old(a[..heapsize])+[itemToAdd])
+    {
+        ghost var a' := a[..heapsize + 1][heapsize := itemToAdd];
+        assert a'[..heapsize] == a[..heapsize];
+        assert a'[..heapsize + 1] == a[..heapsize] + [a'[heapsize]];
+
+        assert multiset(a[..heapsize+1][heapsize := itemToAdd][..heapsize]) == multiset(a[..heapsize]);
+    }
+
+lemma WeakenPrecondForIteration(a : array<int>, heapsize:nat, setToBe : multiset<int>)
+    requires 0 < heapsize <= a.Length
+	requires hp(a[..], heapsize - 1)
+    requires multiset(a[..heapsize]) == setToBe
+
+    ensures  heapsize <= a.Length
+    ensures Inv(a[..], heapsize, heapsize - 1, setToBe)
+    {
+    }
+
+lemma StrengthenPostFromIteration(a : array<int>, heapsize:nat, setToBe : multiset<int>, i : nat)
+    requires Inv(a[..], heapsize, i, setToBe)
+    requires ! (i > 0)
+    ensures hp(a[..], heapsize)
+    ensures multiset(a[..heapsize]) == setToBe
+    {}
+
+method SiftLastItem_Iterate(a : array<int>, heapsize:nat, i0 : nat, ghost setToBe : multiset<int>) returns (i : nat)
+    requires Inv(a[..], heapsize, i0, setToBe)
+
+    ensures Inv(a[..], heapsize, i, setToBe)
+    ensures i == 0
+
+    modifies a
+{
+    i := i0;
+
+     while i > 0
+        invariant Inv(a[..], heapsize, i, setToBe)
+        decreases i
+    {
+        i := LoopBody(a, heapsize, i, setToBe);
+    }
+}
+
+method {:verify true} LoopBody (a : array<int>, heapsize:nat, i0 : nat, ghost setToBe : multiset<int>) returns (i : nat)
+    requires i0 > 0
+    requires Inv(a[..], heapsize, i0, setToBe)
+
+    ensures i < i0
+    ensures Inv(a[..], heapsize, i, setToBe)
+
+    modifies a
+{
+    var ancestor := (i0 - 1) / 2;
+
+    if (a[i0] > a[ancestor])
+    {
+        i := Swap(a, heapsize, i0, setToBe);
+    }
+    else
+    {
+        i := Skip(a, heapsize, i0, setToBe);
+    }
+}
+
+method Swap (a : array<int>, heapsize:nat, i0 : nat, ghost setToBe : multiset<int>) returns (i : nat)
+    requires i0 > 0
+    requires Inv(a[..], heapsize, i0, setToBe)
+    requires a[i0] > a[(i0 - 1) / 2]
+
+    ensures Inv(a[..], heapsize, i, setToBe)
+    ensures i < i0
+
+    modifies a
+    {
+        LemmaSwap(a[..], heapsize, i0, setToBe);
+        a[i0], a[((i0 - 1) / 2)], i := a[(i0 - 1) / 2], a[i0], ((i0 - 1) / 2);
+    } 
+
+method Skip(a : array<int>, heapsize:nat, i0 : nat, ghost setToBe : multiset<int>) returns (i : nat)
+requires i0 > 0
+    requires Inv(a[..], heapsize, i0, setToBe)
+    requires a[i0] <= a[(i0 - 1) / 2]
+
+    ensures Inv(a[..], heapsize, i, setToBe)
+    ensures i < i0
+
+    modifies a
+{
+    LemmaSkip(a[..], heapsize, i0, setToBe);
+    i := (i0 - 1) / 2;
+}
+
+lemma LemmaSkip(a : seq<int>, heapsize:nat, i : nat, setToBe : multiset<int>)
+    requires i > 0
+    requires Inv(a, heapsize, i, setToBe)
+    requires a[i] <= a[(i-1) / 2]
+
+    ensures Inv(a, heapsize, (i-1)/2, setToBe)
+    {
+        ghost var ancestor := (i - 1)/2;
+        assert AncestorIndex(ancestor, i);
+
+        assert forall j :: 
+            i <= j < heapsize &&
+            AncestorIndex(i, j) ==>
+            a[i] >= a[j];
+
+        DirectAncestorLemma(ancestor, i);        
+
+        assert forall j ::
+            0 <= j < i &&
+            AncestorIndex(j, i) ==>
+                AncestorIndex(j, ancestor);
+    }
+
+lemma LemmaSwap(a : seq<int>, heapsize:nat, i : nat, setToBe : multiset<int>)
+    requires i > 0
+    requires Inv(a, heapsize, i, setToBe)
+    requires a[i] > a[(i-1) / 2]
+
+    ensures Inv(a[ i := a[(i-1)/2]][(i-1)/2 := a[i]], heapsize, (i - 1) / 2, setToBe)
+    {
+        ghost var ancestor := (i - 1)/2;
+        assert AncestorIndex(ancestor, i);
+
+        ghost var change1 := a[ i := a[ancestor]];
+        ghost var change2 := change1[ancestor := a[i]];
+
+        assert forall j ::
+            0 <= j < heapsize && 
+            j != i && j != ancestor ==>
+                change2[j] == a[j];
+
+        assert forall j, k ::
+            0 <= j <heapsize &&
+            0 <= k <heapsize &&
+            j != i && j != ancestor &&
+            k != i && k != ancestor &&
+            AncestorIndex(j, k) ==>
+                change2[j] >= change2[k];
+
+        assert forall j ::
+            0 <= j < heapsize && 
+            j != ancestor &&
+            AncestorIndex(i, j) ==>
+                change2[i] >= change2[j];
+
+        DirectAncestorLemma(ancestor, i);
+        
+        assert forall j ::
+            0 <= j < i && 
+            j != ancestor &&
+            AncestorIndex(j, i) ==>
+                change2[j] >= change2[i];
+    
+
+        assert forall j, k ::
+            0 <= j < heapsize && j != ancestor &&
+            0 <= k < heapsize && k != ancestor &&
+            AncestorIndex(j, k) ==>
+                change2[j] >= change2[k];
+
+    }
+
+
+predicate DirectAncestor(ancestor : nat, i : nat)
+{
+    (i - 1) / 2 == ancestor
+}
+
+lemma DirectAncestorLemma(ancestor:nat, i : nat)
+    requires DirectAncestor(ancestor, i)
+    ensures forall j :: ancestor < j < i ==> !AncestorIndex(j, i)  
+    ensures forall j :: 0 <= j < i && j != ancestor ==> (AncestorIndex(j, i) ==> AncestorIndex(j, ancestor))
+
+
+
+method GetAncestorIndex(i : nat) returns (j : nat)
+    requires i >= 1
+    ensures j < i
+    ensures AncestorIndex(j, i)
+{
+    j := ((i - 1) as real / 2 as real).Floor as nat;
+}
